added some proofs in BinaryDefs to make it 'more convincing'

NTCB/BinaryDefs.v
@@ -28,8 +28,7 @@ Lemma half_byte_eq_dec: forall hb1 hb2: half_byte, {hb1 = hb2} + {hb1 <> hb2}.
 Proof. decide equality. Qed.
 
 
-(* TCB *)
-
+Open Scope positive_scope.
 Open Scope N_scope.
 
 Definition half_byte_to_N hb : N:=
@@ -67,7 +66,7 @@ Definition translate_N_by trans (n: N) :=
   end.
 
 (* specialisation for efficiency reasons *)
-Definition translate_N_by_four n := 
+Definition translate_N_by_four n :=
   match n with
     | N0 => N0
     | Npos p => Npos (p~0~0~0~0)
@@ -91,7 +90,6 @@ Qed.
 
 
 
-(* NTCB *)
 
 Definition fst_four_bits n : (half_byte * N) :=
   match n with
@@ -130,8 +128,6 @@ Definition fst_four_bits n : (half_byte * N) :=
   end.
 
 
-(* TCB *)
-
 Definition concat_half_byte n hb := (translate_N_by_four n) + (half_byte_to_N hb).
 
 Lemma fst_four_bits_of_half_byte: forall hb n,
@@ -142,16 +138,17 @@ Qed.
 
 
 
-(* NTCB *)
+
+(* Bytes *)
 
 Definition byte := (half_byte * half_byte)%type.
 
-
-(* TCB *)
-Definition byte_to_N (b: byte) :=
-  (translate_N_by_four (half_byte_to_N (fst b))) + (half_byte_to_N (snd b)).
+Definition byte_to_N (b: byte) : N:=
+  concat_half_byte (half_byte_to_N (fst b)) (snd b).
+(*  (translate_N_by_four (half_byte_to_N (fst b))) + (half_byte_to_N (snd b)).*)
 
 Definition byte0 : byte := (HB0, HB0).
+
 Lemma byte_to_N0: byte_to_N byte0 = 0.
 Proof.
   reflexivity.
@@ -165,6 +162,91 @@ Definition fst_byte n : (byte * N) :=
 Definition concat_byte n (b: byte) :=
   translate_N_by_eight n + byte_to_N b.
 
+(* for proof purpose *)
+Definition concat_byte_aux n (b: byte) :=
+  let (hb2, hb1) := b in
+  let n2 := concat_half_byte n hb2 in
+  concat_half_byte n2 hb1.
+
+
+Lemma translate_P_xO: forall t p, translate_P_by t (p~0) = (translate_P_by t p)~0.
+Proof.
+  induction' t as [|t]; simpl; intros; auto.
+Qed.
+
+Lemma translate_P_plus: forall t1 t2 p, translate_P_by t1 (translate_P_by t2 p) = translate_P_by (t1 + t2) p.
+Proof.
+  induction' t1 as [|t1']; simpl; intros.
+  Case "0%nat".
+    destruct (translate_P_by t2 p); auto.
+  Case "S t1'".
+    repeat rewrite translate_P_xO. f_equal.
+    auto.
+Qed.
+
+Lemma translate_N_plus: forall t1 t2 n, translate_N_by t1 (translate_N_by t2 n) = translate_N_by (t1 + t2) n.
+Proof.
+  intros. destruct n; simpl; auto.
+  f_equal. apply translate_P_plus.
+Qed.
+
+
+
+Lemma translate_N_assoc: forall t n1 n2, translate_N_by t n1 + translate_N_by t n2 = translate_N_by t (n1 + n2).
+Proof.
+  intros.
+  destruct' n1 as [|pos1]; destruct' n2 as [|pos2]; simpl; auto.
+  Case "Npos pos1"; SCase "Npos pos2".
+  f_equal.
+  revert pos1 pos2.
+  induction' t as [|t']; intros; simpl; auto.
+  SSCase "S t'".
+  rewrite IHt'. reflexivity.
+Qed.
+
+
+
+Lemma concat_byte_aux_correct: forall n b,
+  concat_byte n b = concat_byte_aux n b.
+Proof.
+  unfold concat_byte, concat_byte_aux.
+  destruct b as (hb2, hb1).
+  unfold byte_to_N, concat_half_byte. simpl.
+  repeat match goal with
+    | |- context[translate_N_by_four ?n] =>
+      rewrite (translate_N_by_four_correct n)
+  end.
+  repeat match goal with
+    | |- context[translate_N_by_eight ?n] =>
+      rewrite (translate_N_by_eight_correct n)
+  end.
+
+  destruct' n as [|pos].
+  Case "0".
+  simpl. reflexivity.
+  Case "Npos pos".
+  remember (half_byte_to_N hb1) as nhb1. clear Heqnhb1.
+  remember (half_byte_to_N hb2) as nhb2. clear Heqnhb2.
+  rewrite Nplus_assoc. f_equal.
+  rewrite <- (translate_N_plus 4 4).
+  rewrite translate_N_assoc. reflexivity.
+Qed.
+
+
+
+Lemma fst_byte_of_byte: forall b n,
+  fst_byte (concat_byte n b) = (b, n).
+Proof.
+  intros.
+  rewrite concat_byte_aux_correct.
+  destruct b as (hb2, hb1).
+  unfold fst_byte.
+  simpl.
+  repeat rewrite fst_four_bits_of_half_byte. reflexivity.
+Qed.
+
+
+
 
 (* a word is four byte, little endian *)
 Inductive word := W : byte -> byte -> byte -> byte -> word.
@@ -173,16 +255,25 @@ Definition word_to_N w :=
   match w with
     | W b1 b2 b3 b4 =>
       let n4 := byte_to_N b4 in
-      let n3 := translate_N_by_eight n4 + byte_to_N b3 in
-      let n2 := translate_N_by_eight n3 + byte_to_N b2 in
-      translate_N_by_eight n2 + byte_to_N b1
+      let n3 := concat_byte n4 b3 in
+      let n2 := concat_byte n3 b2 in
+      concat_byte n2 b1
   end.
 
-Definition fst_word n :=
+Definition to_word n :=
   let (b1, n1):= fst_byte n in
   let (b2, n2):= fst_byte n1 in
   let (b3, n3):= fst_byte n2 in
   let (b4, n4):= fst_byte n3 in
-  (W b1 b2 b3 b4, n4).
+  W b1 b2 b3 b4.
 
-
+Lemma fst_word_of_word: forall w,
+  to_word (word_to_N w) = w.
+Proof.
+  destruct w as [b1 b2 b3 b4].
+  unfold to_word.
+  simpl. repeat rewrite fst_byte_of_byte.
+  unfold fst_byte, byte_to_N.
+  rewrite fst_four_bits_of_half_byte.
+  destruct b4. simpl. destruct h; reflexivity.
+Qed.
